src/Narcissus/Formats/EnumOpt.v
@@ -8,6 +8,10 @@ Require Import
         Coq.Vectors.Vector
         Bedrock.Word.
 
+Require Import Coq.Strings.String.
+Require Import Fiat.Narcissus.Formats.StringOpt.
+Require Import Fiat.Narcissus.Formats.AsciiOpt.
+
 Section Enum.
   Context {len : nat}.
   Context {A : Type}.
@@ -180,3 +184,147 @@ Ltac Discharge_NoDupVector :=
                  | inversion H]
          end
   end.
+
+Section EnumString.
+  Context {len : nat}.
+  Context {A : Type}.
+  Context {B : Type}.
+  Context {cache : Cache}.
+  Context {cacheAddNat : CacheAdd cache nat}.
+  Context {monoid : Monoid B}.
+  Context {monoidUnit : QueueMonoidOpt monoid bool}.
+
+  Context {ta : t A (S len)}.
+  Variable (tb : t string (S len)).
+
+  Definition space : Ascii.ascii
+    := Ascii.Ascii false false false false false true false false.
+
+  Definition format_enum_string (term_char : Ascii.ascii) (idx : Fin.t _) :
+    CacheFormat -> Comp (B * CacheFormat) :=
+    format_string_with_term_char term_char (nth tb idx).
+
+  Fixpoint string_indexed {n : nat}
+           (w : string)
+           (t : t string n) : option (Fin.t n)
+    := match t in Vector.t _ n return option (Fin.t n) with
+       | nil => None
+       | cons w' _ t' =>
+         if (String.eqb w w') then Some (Fin.F1) else
+           option_map Fin.FS (string_indexed w t')
+       end.
+
+  Fixpoint decode_string (s : nat) (b : B) (cd : CacheDecode) : option (string * B * CacheDecode) :=
+    match s with
+    | O => Some (EmptyString, b, cd)
+    | S s' => `(x, b1, e1) <- decode_ascii b cd;
+               if (Ascii.eqb x " ") then
+                 Some (EmptyString, b1, e1)
+               else
+               `(xs, b2, e2) <- decode_string s' b1 e1;
+                Some (String x xs, b2, e2)
+    end.
+
+  Definition decode_enum_string term_char (b : B)
+             (cd : CacheDecode)
+    : option (Fin.t _ * B * CacheDecode) :=
+    `(w, b', cd') <- (decode_string_with_term_char term_char) b cd;
+      Ifopt string_indexed w tb as idx Then
+      Some (idx, b', cd')
+      Else None.
+
+  Lemma string_indexed_correct :
+    forall n (i : Fin.t n) (t : t string n),
+      NoDupVector t
+      -> match string_indexed (nth t i) t with
+      | Some w' => i = w'
+      | None => False
+      end.
+  Proof.
+    clear.
+    induction i.
+    - intro; pattern n, t; apply Vector.caseS; simpl; intros.
+      rewrite (proj2 (String.eqb_eq h h)); eauto.
+    - intro; generalize i (IHi (Vector.tl t)); clear.
+      pattern n, t; apply Vector.caseS; simpl.
+      intros h n0 t0 i; case_eq (string_indexed (nth t0 i) t0); intros;
+        apply NoDupVector_invert in H1; intuition subst.
+      case_eq (String.eqb (nth t0 t1) h); intros; eauto.
+      apply eqb_eq in H0; subst.
+      destruct H2; generalize t0 H; clear; induction t1.
+      + intro; pattern n, t0; apply Vector.caseS; simpl; intros; econstructor.
+      + intro; revert t1 IHt1; pattern n, t0; apply Vector.caseS;
+          simpl; intros.
+        case_eq (String.eqb (nth t t1) h); intros; eauto.
+        * apply eqb_eq in H0; subst; econstructor.
+        * rewrite H0 in H.
+          econstructor 2; apply IHt1.
+          destruct (string_indexed (nth t t1) t); try discriminate.
+          f_equal.
+          unfold option_map in H.
+          apply Fin.FS_inj; congruence.
+      +
+        unfold option_map; reflexivity.
+  Qed.
+
+  Lemma string_indexed_correct':
+    forall n (v : Fin.t n) (w : string) (t : t string n),
+      string_indexed w t = Some v -> w = nth t v.
+  Proof.
+    clear.
+    induction v.
+    - intros w tb; pattern n, tb;
+        eapply Vector.caseS; simpl.
+      intros; destruct (eqb w h) eqn: ?.
+      eapply eqb_eq; eauto.
+      destruct ( string_indexed w t); try discriminate.
+    - intros w tb.
+      revert w v IHv.
+      pattern n, tb; eapply Vector.rectS; simpl; intros.
+      inversion v.
+      intros; destruct (eqb w a) eqn: ?.
+      discriminate.
+      destruct (string_indexed w v) eqn : ? ; try discriminate.
+      eapply IHv.
+      rewrite Heqo.
+      f_equal.
+      eapply Fin.FS_inj.
+      unfold option_map in H0.
+      congruence.
+  Qed.
+
+  Theorem Enum_decode_string_correct
+          (tb_OK : NoDupVector tb)
+          {P : CacheDecode -> Prop}
+          (P_OK : cache_inv_Property P (fun P => forall b cd, P cd -> P (addD cd b)))
+          term_char
+    : CorrectDecoder monoid
+                     (fun s => forall s1 s2,
+                          (nth tb s) <> s1 ++ String term_char s2)%string
+                     (fun s => forall s1 s2,
+                          (nth tb s) <> s1 ++ String term_char s2)%string
+                     eq
+                     (format_enum_string term_char)
+                     (decode_enum_string term_char) P 
+                     (format_enum_string term_char).
+  Proof.
+    unfold format_enum_string.
+    apply_bijection_rule' with (fun w => string_indexed w tb);
+      intuition eauto using String_decode_with_term_char_correct.
+    eapply string_indexed_correct in tb_OK.
+    destruct string_indexed eqn:?; subst; intuition eauto.
+    symmetry. eauto using string_indexed_correct'; eauto.
+    apply string_indexed_correct' in H0; subst; auto.
+    eapply H; eauto.
+    derive_decoder_equiv.
+    simpl.
+    unfold decode_enum_string.
+    rewrite Heqo.
+    simpl.
+    destruct (string_indexed s tb); auto.
+    unfold decode_enum_string.
+    rewrite Heqo; auto.
+  Defined.
+
+End EnumString.
+
